merging after set header validity changes (#426)
using prodn to streamline shifting operations in lifting pass

vectors

shift_pairs as vec

shifting couples

prodn is hard

good progress on prodn shifting in lifting

lifting refactor

more lifted fixes

lifted refactored

more refactor

fixed more lifting issues

fixed lifting spec proofs

filled holes in liftspec and lifted

builds

coq/lib/P4cub/Semantics/Dynamic/BigStep/Properties.v
@@ -60,7 +60,7 @@ Section Properties.
       ⟨ us ++ ϵ, e ⟩ ⇓ v ->
       ⟨ us ++ vs ++ ϵ,
         shift_exp
-          (Shifter (length us) (length vs)) e ⟩ ⇓ v.
+          (length us) (length vs) e ⟩ ⇓ v.
   Proof using.
     intros us vs ϵ e v h.
     remember (us ++ ϵ) as usϵ eqn:husϵ.
@@ -96,12 +96,12 @@ Section Properties.
   Lemma e_eval_shift : forall e v us vs ϵ,
       ⟨ us ++ vs ++ ϵ,
         shift_exp
-          (Shifter (length us) (length vs)) e ⟩ ⇓ v ->
+          (length us) (length vs) e ⟩ ⇓ v ->
       ⟨ us ++ ϵ, e ⟩ ⇓ v.
   Proof using.
     intro e; induction e using custom_exp_ind;
       intros v us vs eps h; inv h; cbn in *; eauto.
-    - unfold shift_var, cutoff, amt in * |-.
+    - unfold shift_var in * |-.
       destruct_if_hyp.
       + rewrite nth_error_app2 in H3 by lia.
         rewrite <- Nat.add_sub_assoc in H3 by lia.
@@ -128,7 +128,7 @@ Section Properties.
 
   Lemma shift_trns_eval : forall us ϵ p st,
       p⟨ us ++ ϵ , p ⟩ ⇓ st -> forall vs,
-        p⟨ us ++ vs ++ ϵ , shift_trns (Shifter (length us) (length vs)) p ⟩ ⇓ st.
+        p⟨ us ++ vs ++ ϵ , shift_trns (length us) (length vs) p ⟩ ⇓ st.
   Proof using.
     intros us eps p st h vs.
     inv h; unravel; auto.
@@ -137,7 +137,7 @@ Section Properties.
   Local Hint Resolve shift_trns_eval : core.
 
   Lemma trns_eval_shift : forall p st us vs ϵ,
-      p⟨ us ++ vs ++ ϵ , shift_trns (Shifter (length us) (length vs)) p ⟩ ⇓ st ->
+      p⟨ us ++ vs ++ ϵ , shift_trns (length us) (length vs) p ⟩ ⇓ st ->
       p⟨ us ++ ϵ , p ⟩ ⇓ st.
   Proof using.
     intros [lbl | e lbl cases] st us vs eps h; cbn in h; inv h; eauto.
@@ -145,22 +145,22 @@ Section Properties.
 
   Local Hint Resolve trns_eval_shift : core.
   
-  Fixpoint shift_lv (sh : shifter) (lv : Lval.t) : Lval.t :=
+  Fixpoint shift_lv (c a : nat) (lv : Lval.t) : Lval.t :=
   match lv with
-  | Lval.Var x => Lval.Var $ shift_var sh x
-  | Lval.Slice hi lo lv => Lval.Slice hi lo $ shift_lv sh lv
-  | Lval.Member x lv => Lval.Member x $ shift_lv sh lv
-  | Lval.Index n lv => Lval.Index n $ shift_lv sh lv
+  | Lval.Var x => Lval.Var $ shift_var c a x
+  | Lval.Slice hi lo lv => Lval.Slice hi lo $ shift_lv c a lv
+  | Lval.Member x lv => Lval.Member x $ shift_lv c a lv
+  | Lval.Index n lv => Lval.Index n $ shift_lv c a lv
   end.
 
   Lemma shift_lv_0_add : forall lv m n,
-      shift_lv (Shifter 0 (m + n)) lv = shift_lv (Shifter 0 m) (shift_lv (Shifter 0 n) lv).
+      shift_lv 0 (m + n) lv = shift_lv 0 m (shift_lv 0 n lv).
   Proof using.
     intro lv; induction lv; intros m n; unravel; f_equal; auto.
     unfold shift_var; cbn. lia.
   Qed.
   
-  Lemma shift_lv_0 : forall lv c, shift_lv (Shifter c 0) lv = lv.
+  Lemma shift_lv_0 : forall lv c, shift_lv c 0 lv = lv.
   Proof using.
     intros lv c; induction lv; unravel; f_equal; auto.
     unfold shift_var. destruct_if; reflexivity.
@@ -172,8 +172,8 @@ Section Properties.
       l⟨ us ++ ϵ, e ⟩ ⇓ lv ->
       l⟨ us ++ vs ++ ϵ,
           shift_exp
-            (Shifter (length us) (length vs)) e ⟩
-        ⇓ shift_lv (Shifter (length us) (length vs)) lv.
+            (length us) (length vs) e ⟩
+        ⇓ shift_lv (length us) (length vs) lv.
   Proof using.
     intros us vs eps e lv h.
     remember (us ++ eps) as useps eqn:huseps.
@@ -187,13 +187,13 @@ Section Properties.
   Lemma lv_eval_shift : forall e lv us vs ϵ,
       l⟨ us ++ vs ++ ϵ,
           shift_exp
-            (Shifter (length us) (length vs)) e ⟩
-        ⇓ shift_lv (Shifter (length us) (length vs)) lv ->
+            (length us) (length vs) e ⟩
+        ⇓ shift_lv (length us) (length vs) lv ->
       l⟨ us ++ ϵ, e ⟩ ⇓ lv.
   Proof using.
     intro e; induction e using custom_exp_ind;
       intros [] us vs eps h; cbn in *; inv h; eauto.
-    unfold shift_var, cutoff, amt in * |-.
+    unfold shift_var in * |-.
     do 2 destruct_if_hyp; subst; try lia; auto.
     assert (x0 = x) by lia; subst; auto.
   Qed.
@@ -202,8 +202,8 @@ Section Properties.
 
   Lemma shift_exp_lv_eval_shift_lv_exists :
     forall e lv us vs eps,
-      l⟨ us ++ vs ++ eps, shift_exp (Shifter (length us) (length vs)) e ⟩ ⇓ lv -> exists lv',
-        lv = shift_lv (Shifter (length us) (length vs)) lv'.
+      l⟨ us ++ vs ++ eps, shift_exp (length us) (length vs) e ⟩ ⇓ lv -> exists lv',
+        lv = shift_lv (length us) (length vs) lv'.
   Proof.
     intro e; induction e; intros lv us vs eps h;
       unravel in h; inv h; unravel; eauto.
@@ -218,11 +218,11 @@ Section Properties.
   Qed.   
   
   Lemma shift_lv_lookup : forall lv rs us ϵ,
-      lv_lookup (rs ++ us ++ ϵ) (shift_lv (Shifter (length rs) (length us)) lv)
+      lv_lookup (rs ++ us ++ ϵ) (shift_lv (length rs) (length us) lv)
       = lv_lookup (rs ++ ϵ) lv.
   Proof using.
     intro lv; induction lv; intros; unravel.
-    - unfold shift_var, cutoff,amt.
+    - unfold shift_var.
       destruct_if.
       + rewrite nth_error_app2
           with (n := x) by assumption.
@@ -245,13 +245,13 @@ Section Properties.
   Lemma shift_lv_update : forall lv v rs ϵ rs' ϵ',
       length rs = length rs' ->
       lv_update lv v (rs ++ ϵ) = rs' ++ ϵ' -> forall us,
-          lv_update (shift_lv (Shifter (length rs) (length us)) lv) v (rs ++ us ++ ϵ)
+          lv_update (shift_lv (length rs) (length us) lv) v (rs ++ us ++ ϵ)
           = rs' ++ us ++ ϵ'.
   Proof using.
     intro lv; induction lv;
       intros v rs eps rs' eps' hrs hlv us;
       unravel in *; autorewrite with core.
-    - unfold shift_var, cutoff, amt.
+    - unfold shift_var.
       destruct_if.
       + rewrite nth_update_app1 in * by lia.
         replace (length us + x - length rs)
@@ -271,13 +271,13 @@ Section Properties.
 
   Lemma lv_update_shift : forall lv v rs ϵ rs' ϵ' us,
       length rs = length rs' ->
-      lv_update (shift_lv (Shifter (length rs) (length us)) lv) v (rs ++ us ++ ϵ)
+      lv_update (shift_lv (length rs) (length us) lv) v (rs ++ us ++ ϵ)
       = rs' ++ us ++ ϵ' ->
       lv_update lv v (rs ++ ϵ) = rs' ++ ϵ'.
   Proof using.
     intro lv; induction lv;
       intros v rs eps rs' eps' us hrs h; cbn in *.
-    - unfold shift_var,cutoff,amt in * |-.
+    - unfold shift_var in * |-.
       destruct_if_hyp.
       + rewrite app_assoc in h.
         assert (husrsx : length rs + length us <= length us + x) by lia.
@@ -348,8 +348,8 @@ Section Properties.
       arg_big_step (us ++ eps) arg varg ->
       arg_big_step
         (us ++ vs ++ eps)
-        (shift_arg (Shifter (length us) (length vs)) arg)
-        (paramarg_map id (shift_lv (Shifter (length us) (length vs))) varg).
+        (shift_arg (length us) (length vs) arg)
+        (paramarg_map id (shift_lv (length us) (length vs)) varg).
   Proof using.
     unfold arg_big_step.
     intros us vs eps arg varg h; inv h; unravel; auto.
@@ -361,8 +361,8 @@ Section Properties.
       args_big_step (us ++ eps) args vargs ->
       args_big_step
         (us ++ vs ++ eps)
-        (map (shift_arg (Shifter (length us) (length vs))) args)
-        (map (paramarg_map id (shift_lv (Shifter (length us) (length vs)))) vargs).
+        (map (shift_arg (length us) (length vs)) args)
+        (map (paramarg_map id (shift_lv (length us) (length vs))) vargs).
   Proof using.
     unfold args_big_step.
     intros.
@@ -376,8 +376,8 @@ Section Properties.
   Lemma arg_eval_shift : forall us vs eps arg varg,
       arg_big_step
         (us ++ vs ++ eps)
-        (shift_arg (Shifter (length us) (length vs)) arg)
-        (paramarg_map id (shift_lv (Shifter (length us) (length vs))) varg) ->
+        (shift_arg (length us) (length vs) arg)
+        (paramarg_map id (shift_lv (length us) (length vs)) varg) ->
       arg_big_step (us ++ eps) arg varg.
   Proof using.
     unfold arg_big_step.
@@ -389,9 +389,9 @@ Section Properties.
   Lemma arg_eval_shift_exp_exists_shift_varg : forall us vs eps arg varg,
       arg_big_step
         (us ++ vs ++ eps)
-        (shift_arg (Shifter (length us) (length vs)) arg)
+        (shift_arg (length us) (length vs) arg)
         varg ->
-      exists varg', varg = (paramarg_map id (shift_lv (Shifter (length us) (length vs))) varg').
+      exists varg', varg = (paramarg_map id (shift_lv (length us) (length vs)) varg').
   Proof using.
     unfold arg_big_step.
     intros us vs eps [] [] h; unravel in h; inv h; unravel; eauto.
@@ -404,8 +404,8 @@ Section Properties.
   
   Lemma args_eval_shift : forall us vs eps args vargs,
       args_big_step (us ++ vs ++ eps)
-        (map (shift_arg (Shifter (length us) (length vs))) args)
-        (map (paramarg_map id (shift_lv (Shifter (length us) (length vs)))) vargs) ->
+        (map (shift_arg (length us) (length vs)) args)
+        (map (paramarg_map id (shift_lv (length us) (length vs))) vargs) ->
       args_big_step (us ++ eps) args vargs.
   Proof using.
     unfold args_big_step.
@@ -421,9 +421,9 @@ Section Properties.
   Lemma args_eval_shift_exp_exists_shift_varg : forall us vs eps args vargs,
       args_big_step
         (us ++ vs ++ eps)
-        (map (shift_arg (Shifter (length us) (length vs))) args)
+        (map (shift_arg (length us) (length vs)) args)
         vargs -> exists vargs',
-        vargs = (map (paramarg_map id (shift_lv (Shifter (length us) (length vs)))) vargs').
+        vargs = (map (paramarg_map id (shift_lv (length us) (length vs))) vargs').
   Proof using.
     unfold args_big_step.
     intros us vs eps args.
@@ -439,7 +439,7 @@ Section Properties.
     forall us vs eps eps' vargs,
       copy_in vargs (us ++ eps) = Some eps' ->
       copy_in
-        (map (paramarg_map id (shift_lv (Shifter (length us) (length vs)))) vargs)
+        (map (paramarg_map id (shift_lv (length us) (length vs))) vargs)
         (us ++ vs ++ eps) = Some eps'.
   Proof using.
     intros us vs eps eps' vargs h.
@@ -458,7 +458,7 @@ Section Properties.
   Lemma copy_in_shift :
     forall us vs eps eps' vargs,
       copy_in
-        (map (paramarg_map id (shift_lv (Shifter (length us) (length vs)))) vargs)
+        (map (paramarg_map id (shift_lv (length us) (length vs))) vargs)
         (us ++ vs ++ eps) = Some eps' ->
       copy_in vargs (us ++ eps) = Some eps'.
   Proof using.
@@ -518,7 +518,7 @@ Section Properties.
       length us = length us' ->
       copy_out_argv n varg eps'' (us ++ eps) = us' ++ eps' ->
       copy_out_argv
-        n (paramarg_map id (shift_lv (Shifter (length us) (length vs))) varg)
+        n (paramarg_map id (shift_lv (length us) (length vs)) varg)
         eps'' (us ++ vs ++ eps) = us' ++ vs ++ eps'.
   Proof using.
     intros.
@@ -534,7 +534,7 @@ Section Properties.
       length us = length us' ->
       copy_out n vargs eps'' (us ++ eps) = us' ++ eps' ->
       copy_out
-        n (map (paramarg_map id (shift_lv (Shifter (length us) (length vs)))) vargs)
+        n (map (paramarg_map id (shift_lv (length us) (length vs))) vargs)
         eps'' (us ++ vs ++ eps) = us' ++ vs ++ eps'.
   Proof using.
     induction vargs; intros; unravel in *; auto.
@@ -557,13 +557,13 @@ Section Properties.
       length vs = length vs' ->
       (*length eps = length eps' ->*)
       lv_update
-        (shift_lv {| cutoff := Datatypes.length us; amt := Datatypes.length vs |} lv)
+        (shift_lv (length us) (length vs) lv)
         v (us ++ vs ++ eps) = us' ++ vs' ++ eps' ->
       vs = vs'.
   Proof using.
     intro lv; induction lv; intros v us us' vs vs' eps eps' hus hlen h;
       unravel in h.
-    - unfold shift_var,cutoff,amt in h.
+    - unfold shift_var in h.
       destruct_if_hyp.
       + rewrite app_assoc in h.
         assert (length (us ++ vs) <= length vs + x)
@@ -592,7 +592,7 @@ Section Properties.
       length us = length us' ->
       length vs = length vs' ->
       copy_out_argv
-        n (paramarg_map id (shift_lv (Shifter (length us) (length vs))) varg)
+        n (paramarg_map id (shift_lv (length us) (length vs)) varg)
         eps'' (us ++ vs ++ eps) = us' ++ vs' ++ eps' ->
       vs = vs'.
   Proof using.
@@ -607,7 +607,7 @@ Section Properties.
       length us = length us' ->
       length vs = length vs' ->
       copy_out
-        n (map (paramarg_map id (shift_lv (Shifter (length us) (length vs)))) vargs)
+        n (map (paramarg_map id (shift_lv (length us) (length vs))) vargs)
         eps'' (us ++ vs ++ eps) = us' ++ vs' ++ eps' ->
       vs = vs'.
   Proof using.
@@ -615,7 +615,7 @@ Section Properties.
       induction vargs as [| varg vargs ih];
       intros us us' vs vs' eps eps' eps'' n hus hvs h; unravel in h; auto.
     pose proof copy_out_argv_length
-      (paramarg_map id (shift_lv {| cutoff := Datatypes.length us; amt := Datatypes.length vs |}) varg)
+      (paramarg_map id (shift_lv (length us) (length vs)) varg)
       n eps'' (us ++ vs ++ eps) as hlen.
     repeat rewrite app_length in hlen.
     rewrite Nat.add_assoc in hlen.
@@ -632,7 +632,7 @@ Section Properties.
     forall varg us vs eps eps'' eps' us' n,
       length us = length us' ->
       copy_out_argv
-        n (paramarg_map id (shift_lv (Shifter (length us) (length vs))) varg)
+        n (paramarg_map id (shift_lv (length us) (length vs)) varg)
         eps'' (us ++ vs ++ eps) = us' ++ vs ++ eps' ->
       copy_out_argv n varg eps'' (us ++ eps) = us' ++ eps'.
   Proof using.
@@ -647,7 +647,7 @@ Section Properties.
     forall vargs us vs eps eps'' eps' us' n,
       length us = length us' ->
       copy_out
-        n (map (paramarg_map id (shift_lv (Shifter (length us) (length vs)))) vargs)
+        n (map (paramarg_map id (shift_lv (length us) (length vs))) vargs)
         eps''
         (us ++ vs ++ eps) = us' ++ vs ++ eps' ->
       copy_out n vargs eps'' (us ++ eps) = us' ++ eps'.
@@ -655,7 +655,7 @@ Section Properties.
     induction vargs; intros; unravel in *; auto.
     pose proof
       copy_out_argv_length
-      (paramarg_map id (shift_lv (Shifter (length us) (length vs))) a) n eps'' (us ++ vs ++ eps) as h.
+      (paramarg_map id (shift_lv (length us) (length vs)) a) n eps'' (us ++ vs ++ eps) as h.
     repeat rewrite app_length in *.
     rewrite Nat.add_assoc in h.
     apply split_by_length3 in h.
@@ -678,9 +678,9 @@ Section Properties.
       lv_update_signal olv sig (copy_out 0 vargs eps'' (us ++ eps))
       = us' ++ eps' ->
       lv_update_signal
-        (option_map (shift_lv (Shifter (length us) (length vs))) olv)
+        (option_map (shift_lv (length us) (length vs)) olv)
         sig
-        (copy_out 0 (map (paramarg_map id (shift_lv (Shifter (length us) (length vs)))) vargs)
+        (copy_out 0 (map (paramarg_map id (shift_lv (length us) (length vs))) vargs)
            eps'' (us ++ vs ++ eps))
       = us' ++ vs ++ eps'.
   Proof using.
@@ -712,9 +712,9 @@ Section Properties.
     forall olv sig vargs us eps eps' us' vs eps'',
       length us = length us' ->
       lv_update_signal
-        (option_map (shift_lv (Shifter (length us) (length vs))) olv)
+        (option_map (shift_lv (length us) (length vs)) olv)
         sig
-        (copy_out 0 (map (paramarg_map id (shift_lv (Shifter (length us) (length vs)))) vargs)
+        (copy_out 0 (map (paramarg_map id (shift_lv (length us) (length vs))) vargs)
            eps'' (us ++ vs ++ eps))
       = us' ++ vs ++ eps' ->
       lv_update_signal olv sig (copy_out 0 vargs eps'' (us ++ eps))
@@ -724,7 +724,7 @@ Section Properties.
     intros [lv |] [] vargs us eps eps' us' vs eps'' hus h; unravel in *; eauto.
     destruct v as [v |]; unravel in *; eauto.
     pose proof copy_out_length
-      (map (paramarg_map id (shift_lv {| cutoff := Datatypes.length us; amt := Datatypes.length vs |})) vargs)
+      (map (paramarg_map id (shift_lv (length us) (length vs))) vargs)
       0 eps'' (us ++ vs ++ eps) as H.
     repeat rewrite app_length in H.
     rewrite Nat.add_assoc in H.
@@ -744,9 +744,9 @@ Section Properties.
       length us = length us' ->
       length vs = length vs' ->
       lv_update_signal
-        (option_map (shift_lv (Shifter (length us) (length vs))) olv)
+        (option_map (shift_lv (length us) (length vs)) olv)
         sig
-        (copy_out 0 (map (paramarg_map id (shift_lv (Shifter (length us) (length vs)))) vargs)
+        (copy_out 0 (map (paramarg_map id (shift_lv (length us) (length vs))) vargs)
            eps'' (us ++ vs ++ eps))
       = us' ++ vs' ++ eps' ->
       vs = vs'.
@@ -755,7 +755,7 @@ Section Properties.
       unravel in *; eauto 2.
     destruct v; eauto 2.
     pose proof copy_out_length
-      (map (paramarg_map id (shift_lv {| cutoff := Datatypes.length us; amt := Datatypes.length vs |})) vargs)
+      (map (paramarg_map id (shift_lv (length us) (length vs))) vargs)
       0 eps'' (us ++ vs ++ eps) as H.
     repeat rewrite app_length in H.
     rewrite Nat.add_assoc in H.
@@ -798,7 +798,7 @@ Section Properties.
       ctx_cutoff (length ϵ) c ->
       ⧼ Ψ , us ++ ϵ , c , s ⧽ ⤋ ⧼ us' ++ ϵ' , sig , ψ ⧽ -> forall vs,
           ⧼ Ψ , us ++ vs ++ ϵ , c ,
-            shift_stm (Shifter (length us) (length vs)) s ⧽
+            shift_stm (length us) (length vs) s ⧽
             ⤋ ⧼ us' ++ vs ++ ϵ' , sig , ψ ⧽.
   Proof using.
     intros Psi us us' eps eps' c s sig psi hus hc hs.
@@ -868,16 +868,16 @@ Section Properties.
     - pose proof shift_lv_update _ _ _ _ _ _ hus huseps' vs0 as hvs.
       rewrite <- hvs. eauto.
     - set (vargs' :=
-             map (paramarg_map id (shift_lv
-                                     {|
-                                       cutoff := Datatypes.length us;
-                                       amt := Datatypes.length vs
-                                     |})) vargs) in *.
+             map
+               (paramarg_map
+                  id
+                  (shift_lv
+                     (length us)
+                     (length vs))) vargs) in *.
       set (olv' :=
-             option_map (shift_lv
-             {|
-               cutoff := Datatypes.length us; amt := Datatypes.length vs
-             |}) olv) in *.      
+             option_map
+               (shift_lv
+                  (length us) (length vs)) olv) in *.
       replace (us' ++ vs ++ eps')
         with (lv_update_signal olv' sig (copy_out 0 vargs' ϵ'' (us ++ vs ++ eps))).
       eapply sbs_funct_call; eauto using shift_args_eval, shift_copy_in.
@@ -886,7 +886,7 @@ Section Properties.
         erewrite shift_lv_update_signal; eauto.
     - replace (us' ++ vs ++ eps')
         with (copy_out 0
-                (map (paramarg_map id (shift_lv (Shifter (length us) (length vs)))) vdata_args)
+                (map (paramarg_map id (shift_lv (length us) (length vs))) vdata_args)
                 ϵ''
                 (us ++ vs ++ eps)) by eauto.
       eapply sbs_action_call; try eassumption; eauto 3.
@@ -898,14 +898,14 @@ Section Properties.
       admit.
     - replace (us' ++ vs ++ eps')
         with (copy_out 0
-                (map (paramarg_map id (shift_lv (Shifter (length us) (length vs)))) vargs)
+                (map (paramarg_map id (shift_lv (length us) (length vs))) vargs)
                 ϵ''
                 (us ++ vs ++ eps)) by eauto.
       econstructor; eauto.
     - (* parser case... *)
       replace (us' ++ vs ++ eps')
         with (copy_out 0
-                (map (paramarg_map id (shift_lv (Shifter (length us) (length vs)))) vargs)
+                (map (paramarg_map id (shift_lv (length us) (length vs))) vargs)
                 ϵ''
                 (us ++ vs ++ eps)) by eauto.
       econstructor; eauto.
@@ -943,8 +943,8 @@ Section Properties.
   Lemma relop_lexp_big_step_exists_shift : forall us vs eps oe olv,
       relop
         (lexp_big_step (us ++ vs ++ eps))
-        (option_map (shift_exp (Shifter (length us) (length vs))) oe) olv -> exists olv',
-        olv = option_map (shift_lv (Shifter (length us) (length vs))) olv'.
+        (option_map (shift_exp (length us) (length vs)) oe) olv -> exists olv',
+        olv = option_map (shift_lv (length us) (length vs)) olv'.
   Proof using.
     intros us vs eps oe olv h.
     destruct oe as [e |]; destruct olv as [lv |]; unravel in *; inv h.
@@ -958,7 +958,7 @@ Section Properties.
       length vs = length vs' ->
       ctx_cutoff (length ϵ) c ->
       ⧼ Ψ , us ++ vs ++ ϵ , c ,
-        shift_stm (Shifter (length us) (length vs)) s ⧽
+        shift_stm (length us) (length vs) s ⧽
         ⤋ ⧼ us' ++ vs' ++ ϵ' , sig , ψ ⧽ ->
       vs = vs'.
   Proof using.
@@ -999,8 +999,7 @@ Section Properties.
     - apply args_eval_shift_exp_exists_shift_varg in H3 as [vargs' ?]; subst.
       apply copy_out_shift_amt in H1; eauto 2.
     - admit.
-    - unfold shext,smother,RecordSet.set,cutoff,amt in *.
-      replace (1 + length us) with (length (v :: us)) in H8 by reflexivity.
+    - replace (1 + length us) with (length (v :: us)) in H8 by reflexivity.
       replace (v :: us ++ vs ++ eps) with ((v :: us) ++ vs ++ eps) in H8 by reflexivity.
       replace (v' :: us' ++ vs' ++ eps') with ((v' :: us') ++ vs' ++ eps') in H8 by reflexivity.
       apply IHs in H8; cbn; auto; lia.
@@ -1028,7 +1027,7 @@ Section Properties.
       length us = length us' ->
       ctx_cutoff (length ϵ) c ->
       ⧼ Ψ , us ++ vs ++ ϵ , c ,
-        shift_stm (Shifter (length us) (length vs)) s ⧽
+        shift_stm (length us) (length vs) s ⧽
         ⤋ ⧼ us' ++ vs ++ ϵ' , sig , ψ ⧽ ->
       ⧼ Ψ , us ++ ϵ , c , s ⧽ ⤋ ⧼ us' ++ ϵ' , sig , ψ ⧽.
   Proof using.
@@ -1082,7 +1081,6 @@ Section Properties.
       econstructor; eauto.
     - admit.
     - pose proof IHs Psi (v :: us) (v' :: us') vs eps eps' c sig psi ltac:(cbn; lia) as ih.
-      unfold shext,smother,RecordSet.set,cutoff,amt in H8. cbn in H8, ih.
       destruct init as [t | e]; inv H7; eauto.
     - pose proof sbs_length _ _ _ _ _ _ _ H3 as hlen1.
       pose proof sbs_length _ _ _ _ _ _ _ H7 as hlen2.
