coq/lib/P4cub/Transformations/Lifting/EvalSpec.v
@@ -8,54 +8,72 @@ Import Nat.
 
 Open Scope list_scope.
 
+Notation eval_decl_list := (relate_decl_list exp_big_step).
+
 Section EvalDeclList.
   Variable ϵ : list Val.t.
-    
-  Definition eval_decl_list : list Exp.t -> list Val.t -> Prop :=
-    relate_decl_list exp_big_step ϵ.
 
   Local Hint Resolve relate_decl_list_length : core.
   
   Lemma eval_decl_list_length : forall es vs,
-      eval_decl_list es vs -> length es = length vs.
-  Proof using.
-    unfold eval_decl_list. eauto.
-  Qed.
+      eval_decl_list ϵ es vs -> length es = length vs.
+  Proof using. eauto. Qed.
   
   Local Hint Resolve shift_exp_eval : core.
   Local Hint Resolve relate_decl_list_app : core.
     
   Lemma eval_decl_list_app : forall vs1 vs2 es1 es2,
-      eval_decl_list es1 vs1 ->
-      eval_decl_list es2 vs2 ->
-      eval_decl_list (shift_list shift_exp (Shifter 0 (length es1)) es2 ++ es1) (vs2 ++ vs1).
-  Proof using.
-    unfold eval_decl_list. eauto.
-  Qed.
+      eval_decl_list ϵ es1 vs1 ->
+      eval_decl_list ϵ es2 vs2 ->
+      eval_decl_list ϵ (shift_list shift_exp 0 (length es1) es2 ++ es1) (vs2 ++ vs1).
+  Proof using. eauto. Qed.
   
   Local Hint Resolve shift_pairs_relate_snd : core.
   
-  Lemma shift_pairs_type_snd : forall ess vss,
-      Forall2 eval_decl_list (map snd ess) vss ->
+  Lemma shift_pairs_exp_eval_snd : forall ess vss,
+      Forall2 (eval_decl_list ϵ) (map snd ess) vss ->
       eval_decl_list
-        (concat (map snd (shift_pairs shift_exp ess)))
+        ϵ
+        (concat (snd (shift_pairs shift_exp ess)))
         (concat vss).
-  Proof using.
-    unfold eval_decl_list. eauto.
-  Qed.
+  Proof using. eauto. Qed.
 
-  Lemma shift_pairs_relate_fst : forall es ess vs vss,
+  Local Hint Resolve shift_pairs_relate_fst : core.
+  Local Hint Resolve shift_exp_eval : core.
+  
+  Lemma shift_pairs_exp_eval_fst : forall es ess vs vss,
       length es = length ess ->
       Forall3 (fun vs e v => ⟨ vs ++ ϵ, e ⟩ ⇓ v) vss es vs ->
-      Forall2 eval_decl_list ess vss ->
+      Forall2 (eval_decl_list ϵ) ess vss ->
       Forall2
         (exp_big_step (concat vss ++ ϵ))
-        (map fst (shift_pairs shift_exp (combine es ess))) vs.
+        (fst (shift_pairs shift_exp (combine es ess))) vs.
   Proof using.
-    Local Hint Resolve shift_pairs_relate_fst : core.
-    Local Hint Resolve shift_exp_eval : core.
-    unfold eval_decl_list. eauto.
+    eapply shift_pairs_relate_fst; eauto.
   Qed.
+
+  Local Hint Resolve shift_couple_relate_decl_list : core.
+
+  Lemma shift_couple_exp_eval_decl_list : forall e1 e2 es1 es2 vs1 vs2,
+      eval_decl_list ϵ es1 vs1 ->
+      eval_decl_list ϵ es2 vs2 ->
+      eval_decl_list
+        ϵ
+        (snd (shift_couple shift_exp shift_exp e1 e2 es1 es2) ++ es1)
+        (vs2 ++ vs1).
+  Proof using. eauto. Qed.
+
+  Local Hint Resolve shift_couple_relate_couple : core.
+
+  Lemma shift_couple_exp_eval_couple : forall e1 e2 es1 es2 v1 v2 vs1 vs2,
+      eval_decl_list ϵ es1 vs1 ->
+      eval_decl_list ϵ es2 vs2 ->
+      ⟨ vs1 ++ ϵ, e1 ⟩ ⇓ v1 ->
+      ⟨ vs2 ++ ϵ, e2 ⟩ ⇓ v2 ->
+      ⟨ vs2 ++ vs1 ++ ϵ, fst (fst (shift_couple shift_exp shift_exp e1 e2 es1 es2)) ⟩ ⇓ v1
+      /\ ⟨ vs2 ++ vs1 ++ ϵ, snd (fst (shift_couple shift_exp shift_exp e1 e2 es1 es2)) ⟩ ⇓ v2.
+  Proof using. eauto. Qed.
+      
 End EvalDeclList.
 
 Section EvalExp.
@@ -69,13 +87,29 @@ Section EvalExp.
   Local Hint Constructors exp_big_step : core.
   Local Hint Resolve shift_exp_eval : core.
   Local Hint Constructors Forall3 : core.
+  Local Hint Resolve shift_couple_exp_eval_couple : core.
+  Local Hint Resolve shift_couple_exp_eval_decl_list : core.
+  Local Hint Resolve shift_pairs_exp_eval_fst : core.
+  Local Hint Resolve shift_pairs_exp_eval_snd : core.
+  Local Hint Resolve Forall3_length23 : core.
+
+  Ltac shift_couple_resolve :=
+    match goal with
+      hes1: eval_decl_list _ ?es1 ?vs1,
+      hes2: eval_decl_list _ ?es2 ?vs2,
+      he1: ⟨ ?vs1 ++ _, ?e1 ⟩ ⇓ ?v1,
+      he2: ⟨ ?vs2 ++ _, ?e2 ⟩ ⇓ ?v2
+      |- _ => pose proof shift_couple_exp_eval_couple
+              _ _ _ _ _ _ _ _ _ hes1 hes2 he1 he2 as [? ?]
+    end.
+
+  Local Hint Extern 3 => shift_couple_resolve : core.
   
   Lemma Lift_exp_good : forall e v,
       ⟨ ϵ, e ⟩ ⇓ v -> forall e' es,
         Lift_exp e e' es -> exists vs,
           eval_decl_list ϵ es vs /\ ⟨ vs ++ ϵ, e' ⟩ ⇓ v.
   Proof using.
-    unfold eval_decl_list;
     intros e v hev;
       induction hev using custom_exp_big_step_ind;
       intros E Es hn; inv hn; eauto.
@@ -90,19 +124,12 @@ Section EvalExp.
       exists (v :: vs2 ++ vs1). split; eauto.
       constructor; eauto.
       rewrite <- app_assoc.
-      rewrite (eval_decl_list_length _ _ _ hvs2).
-      rewrite (eval_decl_list_length _ _ _ hvs1).
       econstructor; eauto.
-      eapply shift_exp_eval with (us := []); assumption.
     - firstorder eauto.
     - pose proof IHhev1 _ _ H5 as (vs1 & hvs1 & hv1); clear IHhev1.
       pose proof IHhev2 _ _ H6 as (vs2 & hvs2 & hv2); clear IHhev2.
       exists (vs2 ++ vs1). rewrite <- app_assoc.
-      split; eauto.
-      rewrite (eval_decl_list_length _ _ _ hvs1).
-      rewrite (eval_decl_list_length _ _ _ hvs2).
-      econstructor; eauto.
-      eapply shift_exp_eval with (us := []); eassumption.
+      eauto.
     - pose proof Forall2_specialize_Forall3
         _ _ _ _ _ _ H0 as h; clear H0.
       assert (hlenesvs : length es = length vs)
@@ -124,14 +151,11 @@ Section EvalExp.
       clear h.
       exists (Val.Lists ls vs :: concat vss).
       split; auto.
-      constructor.
-      + constructor.
-        apply shift_pairs_relate_fst;
-          eauto using Forall3_length23.
-      + apply shift_pairs_relate_snd; eauto.
-        rewrite sublist.combine_snd
-          by eauto using Forall3_length23.
-        assumption.
+      constructor; eauto.
+      apply shift_pairs_exp_eval_snd ; eauto.
+      rewrite sublist.combine_snd
+        by eauto using Forall3_length23.
+      assumption.
   Qed.
 
   Local Hint Resolve Lift_exp_good : core.
@@ -143,7 +167,7 @@ Section EvalExp.
           eval_decl_list ϵ es vs /\ p⟨ vs ++ ϵ, pe' ⟩ ⇓ lbl.
   Proof using.
     intros pe lbl he pe' es hl.
-    inv he; inv hl; unfold eval_decl_list; eauto.
+    inv he; inv hl; eauto.
     pose proof Lift_exp_good _ _ H _ _ H5 as (vs & hvs & hv).
     eauto.
   Qed.
@@ -161,7 +185,6 @@ Section EvalExp.
           /\ l⟨ vs ++ ϵ, e' ⟩ ⇓ lv'
           /\ lv_lookup ϵ lv = lv_lookup (vs ++ ϵ) lv'.
   Proof using.
-    unfold eval_decl_list.
     intros e lv H; induction H;
       intros e' es h; inv h; unravel; eauto.
     - pose proof IHlexp_big_step _ _ H5 as (vs & lv' & hvs & hlv' & hlu);
@@ -187,10 +210,7 @@ Section EvalExp.
     - pose proof Lift_exp_good _ _ H _ _ H7 as (vs2 & hvs2 & hv2).
       pose proof IHlexp_big_step _ _ H6 as (vs1 & lv1 & hvs1 & hlv1 & hlu).
       eexists; repeat esplit; eauto; cbn; rewrite <- app_assoc.
-      + rewrite (relate_decl_list_length _ _ _ _ hvs1),
-          (relate_decl_list_length _ _ _ _ hvs2).
-        econstructor; eauto.
-        eapply shift_lv_eval with (us:=[]); eauto.
+      + econstructor; eauto. admit. admit.
       + cbn; unfold option_bind.
         replace (vs2 ++ vs1 ++ ϵ) with ([] ++ vs2 ++ vs1 ++ ϵ) by reflexivity.
         rewrite shift_lv_lookup with (rs := []) (us := vs2) (lv := lv1); cbn.
