coq/lib/P4cub/Transformations/Lifting/Lift.v
@@ -5,6 +5,7 @@ From Poulet4 Require Import
      P4cub.Syntax.CubNotations P4cub.Syntax.Shift
      P4cub.Syntax.IndPrincip
      P4cub.Transformations.Lifting.Statementize
+     P4cub.Transformations.Lifting.LiftList
      Utils.ForallMap.
 Import ListNotations Nat.
 From RecordUpdate Require Import RecordSet.
@@ -12,36 +13,6 @@ Import RecordSetNotations.
 
 Local Open Scope exp_scope.
 Local Open Scope stm_scope.
-
-Goal forall e es,
-    shift_pairs shift_exp [(e,es)] = [(e,es)].
-Proof.
-  intros; cbn; rewrite shift_exp_0 , shift_explist_0. reflexivity.
-Qed.
-
-Goal forall e1 e2 es1 es2,
-    shift_pairs shift_exp [(e2,es2);(e1,es1)]
-    = [(shift_exp (Shifter (length es2) (length es1)) e2,
-         shift_list shift_exp (Shifter 0 (length es1)) es2);
-       (shift_exp (Shifter 0 (length es2)) e1, es1)].
-Proof.
-  intros; unravel.
-  rewrite add_0_r, shift_explist_0, shift_exp_0.
-  reflexivity.
-Qed.
-
-Goal forall e1 e2 e3 es1 es2 es3,
-    shift_pairs shift_exp [(e3,es3);(e2,es2);(e1,es1)]
-    = [(shift_exp (Shifter (length es3) (length es2 + length es1)) e3,
-            shift_list shift_exp (Shifter 0 (length es2 + length es1)) es3);
-       (shift_exp (Shifter 0 (length es3)) (shift_exp (Shifter (length es2) (length es1)) e2),
-         shift_list shift_exp (Shifter 0 (length es1)) es2);
-       (shift_exp (Shifter 0 (length es3 + length es2)) e1, es1)].
-Proof.
-  intros; unravel.
-  rewrite add_0_r, shift_explist_0, shift_exp_0, shift_exp_add.
-  reflexivity.
-Qed.
 
 Inductive Lift_exp
   : Exp.t -> Exp.t -> list Exp.t -> Prop :=
@@ -79,9 +50,9 @@ Inductive Lift_exp
     (Exp.Index t e1 e2)
     (Exp.Index
        t
-       (shift_exp (Shifter 0 (length es2)) e1')
-       (shift_exp (Shifter (length es2) (length es1)) e2'))
-    (shift_list shift_exp (Shifter 0 (length es1)) es2 ++ es1)
+       (fst (fst (shift_couple shift_exp shift_exp e1' e2' es1 es2)))
+       (snd (fst (shift_couple shift_exp shift_exp e1' e2' es1 es2))))
+    (snd (shift_couple shift_exp shift_exp e1' e2' es1 es2) ++ es1)
 | Lift_bop t o e1 e2 e1' e2' es1 es2 :
   Lift_exp e1 e1' es1 ->
   Lift_exp e2 e2' es2 ->
@@ -90,16 +61,16 @@ Inductive Lift_exp
     (Exp.Var t "lifted_bop" 0)
     (Exp.Bop
        t o
-       (shift_exp (Shifter 0 (length es2)) e1')
-       (shift_exp (Shifter (length es2) (length es1)) e2')
-       :: shift_list shift_exp (Shifter 0 (length es1)) es2 ++ es1)
+       (fst (fst (shift_couple shift_exp shift_exp e1' e2' es1 es2)))
+       (snd (fst (shift_couple shift_exp shift_exp e1' e2' es1 es2)))
+       :: snd (shift_couple shift_exp shift_exp e1' e2' es1 es2) ++ es1)
 | Lift_lists ls es es' ess :
   Forall3 Lift_exp es es' ess ->
   Lift_exp
     (Exp.Lists ls es)
     (Exp.Var (typ_of_lists ls es) "lifted_lists" 0)
-    (Exp.Lists ls (map fst (shift_pairs shift_exp (combine es' ess)))
-       :: concat (map snd (shift_pairs shift_exp (combine es' ess)))).
+    (Exp.Lists ls (fst (shift_pairs shift_exp (combine es' ess)))
+       :: concat (snd (shift_pairs shift_exp (combine es' ess)))).
 
 Section LifteInduction.
   Variable P : Exp.t -> Exp.t -> list Exp.t -> Prop.
@@ -153,9 +124,9 @@ Section LifteInduction.
         (Exp.Index t e1 e2)
         (Exp.Index
            t
-           (shift_exp (Shifter 0 (length es2)) e1')
-           (shift_exp (Shifter (length es2) (length es1)) e2'))
-        (shift_list shift_exp (Shifter 0 (length es1)) es2 ++ es1).
+           (fst (fst (shift_couple shift_exp shift_exp e1' e2' es1 es2)))
+           (snd (fst (shift_couple shift_exp shift_exp e1' e2' es1 es2))))
+        (snd (shift_couple shift_exp shift_exp e1' e2' es1 es2) ++ es1).
   
   Hypothesis HLift_bop : forall t o e1 e2 e1' e2' es1 es2,
       Lift_exp e1 e1' es1 ->
@@ -167,9 +138,9 @@ Section LifteInduction.
         (Exp.Var t "lifted_bop" 0)
         (Exp.Bop
            t o
-           (shift_exp (Shifter 0 (length es2)) e1')
-           (shift_exp (Shifter (length es2) (length es1)) e2')
-           :: shift_list shift_exp (Shifter 0 (length es1)) es2 ++ es1).
+           (fst (fst (shift_couple shift_exp shift_exp e1' e2' es1 es2)))
+           (snd (fst (shift_couple shift_exp shift_exp e1' e2' es1 es2)))
+           :: snd (shift_couple shift_exp shift_exp e1' e2' es1 es2) ++ es1).
   
   Hypothesis HLift_lists : forall ls es es' ess,
       Forall3 Lift_exp es es' ess ->
@@ -177,8 +148,8 @@ Section LifteInduction.
       P
         (Exp.Lists ls es)
         (Exp.Var (typ_of_lists ls es) "lifted_lists" 0)
-        (Exp.Lists ls (map fst (shift_pairs shift_exp (combine es' ess)))
-           :: concat (map snd (shift_pairs shift_exp (combine es' ess)))).
+        (Exp.Lists ls (fst (shift_pairs shift_exp (combine es' ess)))
+           :: concat (snd (shift_pairs shift_exp (combine es' ess)))).
 
   Definition custom_Lift_exp_ind : forall e e' es,
       Lift_exp e e' es -> P e e' es :=
@@ -251,11 +222,11 @@ Variant Lift_call :
       (Call.Method ext mtd τs (Some e))
       (Call.Method ext mtd τs (Some e')) es
   | Lift_action_call a cargs cargs' ess :
-    Forall3 Lift_exp cargs cargs' ess ->
+    Lift_A_list shift_exp Lift_exp cargs cargs' ess ->
     Lift_call
       (Call.Action a cargs)
-      (Call.Action a (map fst (shift_pairs shift_exp (combine cargs' ess))))
-      (concat (map snd (shift_pairs shift_exp (combine cargs' ess))))
+      (Call.Action a cargs')
+      ess
   | Lift_inst_call x eargs :
     Lift_call (Call.Inst x eargs) (Call.Inst x eargs) [].
 
@@ -282,9 +253,9 @@ Inductive Lift_stm : Stm.t -> Stm.t -> Prop :=
   Lift_stm
     (e1 `:= e2)
     (Unwind
-       (shift_list shift_exp (Shifter 0 (length es1)) es2 ++ es1)
-       (shift_exp (Shifter 0 (length es2)) e1'
-          `:= shift_exp (Shifter (length es2) (length es1)) e2'))
+       (snd (shift_couple shift_exp shift_exp e1' e2' es1 es2) ++ es1)
+       (fst (fst (shift_couple shift_exp shift_exp e1' e2' es1 es2))
+          `:= snd (fst (shift_couple shift_exp shift_exp e1' e2' es1 es2))))
 | Lift_setvalidity b e e' es :
   Lift_exp e e' es ->
   Lift_stm (Stm.SetValidity b e) (Unwind es (Stm.SetValidity b e'))
@@ -295,18 +266,17 @@ Inductive Lift_stm : Stm.t -> Stm.t -> Prop :=
   Lift_stm
     (Stm.Invoke (Some e) t)
     (Unwind es (Stm.Invoke (Some e') t))
-| Lift_app fk fk' fkes args args' argsess :
+| Lift_app fk fk' fkes args args' argses :
   Lift_call fk fk' fkes ->
-  Forall3 Lift_arg args args' argsess ->
+  Lift_A_list shift_arg Lift_arg args args' argses ->
   Lift_stm
     (Stm.App fk args)
     (Unwind
-       (shift_list shift_exp (Shifter 0 (length (concat argsess))) fkes
-          ++ concat (map snd (shift_pairs shift_arg (combine args' argsess))))
+       (snd (shift_couple (fun c a => map (shift_arg c a)) shift_call args' fk' argses fkes)
+          ++ argses)
        (Stm.App
-           (shift_call (Shifter (length fkes) (length (concat argsess))) fk')
-           (map (shift_arg $ Shifter 0 (length fkes))
-              (map fst (shift_pairs shift_arg (combine args' argsess))))))
+           (snd (fst (shift_couple (fun c a => map (shift_arg c a)) shift_call args' fk' argses fkes)))
+           (fst (fst (shift_couple (fun c a => map (shift_arg c a)) shift_call args' fk' argses fkes)))))
 | Lift_stmeq s1 s2 s1' s2' :
   Lift_stm s1 s1' ->
   Lift_stm s2 s2' ->
@@ -320,8 +290,8 @@ Inductive Lift_stm : Stm.t -> Stm.t -> Prop :=
     (Unwind
        es
        (`if e'
-          `then shift_stm (Shifter 0 (length es)) s1'
-          `else shift_stm (Shifter 0 (length es)) s2'))
+          `then shift_stm 0 (length es) s1'
+          `else shift_stm 0 (length es) s2'))
 | Lift_var_typ og t s s' :
   Lift_stm s s' ->
   Lift_stm
@@ -333,23 +303,7 @@ Inductive Lift_stm : Stm.t -> Stm.t -> Prop :=
     (`let og := inr e `in s)
     (Unwind
        es
-       (`let og := inr e' `in shift_stm (Shifter 1 (length es)) s')).
-
-Ltac destr_call_pair f :=
-  match goal with
-  | |- context [f ?a]
-    => destruct (f a) as [? ?] eqn:?; subst
-  end.
-    
-Ltac destr_lift_exp := destr_call_pair lift_exp.
-
-Ltac destr_lift_arg := destr_call_pair lift_arg.
-
-Ltac destr_lift_exp_list := destr_call_pair lift_exp_list.
-
-Ltac destr_lift_trns := destr_call_pair lift_trns.
-
-Ltac destr_lift_args := destr_call_pair lift_args.
+       (`let og := inr e' `in shift_stm 1 (length es) s')).
 
 Section Liftlift.
   Lemma Lift_lift_exp : forall e e' es,
@@ -358,13 +312,9 @@ Section Liftlift.
     intros e e' es h;
       induction h using custom_Lift_exp_ind;
       unravel;
-      repeat destr_lift_exp;
-      repeat match goal with
-        | h: (_, _) = (_, _) |- _ => inv h
-        end; auto.
-    destruct (split (shift_pairs shift_exp (map lift_exp es)))
-      as [es'' les] eqn:hsplit.
-    rewrite split_map in hsplit. inv hsplit.
+      repeat let_destr_pair;
+      repeat pair_fst_snd_eqns;
+      auto.
     enough (map lift_exp es = combine es' ess) as h.
     { do 5 f_equal; assumption. }
     assert (h12 : length es = length es') by eauto using Forall3_length12.
@@ -429,8 +379,7 @@ Section Liftlift.
       Forall3 Lift_exp es es' ess ->
       map lift_exp es = combine es' ess.
   Proof.
-    intros es es' ess h;
-      induction h; cbn; f_equal; auto.
+    refine (Forall3_LiftA_map_lifta _ _ _). auto.
   Qed.
 
   Ltac apply_Forall3_Lift_lift_exp :=
@@ -445,12 +394,11 @@ Section Liftlift.
       Lift_call fk fk' es ->
       lift_call fk = (fk', es).
   Proof.
-    intros fk fk' es h; inv h; unravel; auto.
+    intros fk fk' es h; inv h; cbn; auto.
+    let_destr_pair.
+    eapply Lift_A_list_lift_A_list with (lifta:=lift_exp) in H; auto.
     unfold lift_exp_list.
-    destruct (split (shift_pairs shift_exp $ map lift_exp cargs))
-      as [es les] eqn:hs.
-    rewrite split_map in hs; unravel in hs; inv hs.
-    auto.
+    pair_fst_snd_eqns. reflexivity.
   Qed.
 
   Local Hint Resolve Lift_lift_call : core.
@@ -467,8 +415,7 @@ Section Liftlift.
       Forall3 Lift_arg args args' ess ->
       map lift_arg args = combine args' ess.
   Proof.
-    intros es es' ess h;
-      induction h; cbn; f_equal; auto.
+    refine (Forall3_LiftA_map_lifta _ _ _). auto.
   Qed.
 
   Ltac apply_Forall3_Lift_lift_arg :=
@@ -482,25 +429,11 @@ Section Liftlift.
   Lemma Lift_lift_stm : forall s s',
       Lift_stm s s' -> lift_stm s = s'.
   Proof.
-    intros s s' h; induction h; unravel; subst; auto.
-    - apply_Lift_lift_call.
-      unfold lift_args.
-      destruct
-        (split (shift_pairs shift_arg $ map lift_arg args))
-        as [Args les] eqn:hsplit.
-      rewrite split_map in hsplit.
-      unravel in *; inv hsplit.
-      rewrite sublist.length_concat.
-      rewrite shift_pairs_inner_length.
-      rewrite <- sublist.length_concat.
-      assert (hlen12 : length args = length args')
-        by eauto using Forall3_length12.
-      assert (hlen13 : length args = length argsess)
-        by eauto using Forall3_length13.
-      assert (hlen23 : length args' = length argsess)
-        by eauto using Forall3_length23.
-      apply_Forall3_Lift_lift_arg.
-      repeat f_equal; auto using map_snd_combine.
+    intros s s' h; induction h; unravel; subst;
+      repeat let_destr_pair; auto.
+    apply Lift_lift_call in H.
+    apply Lift_A_list_lift_A_list with (lifta:=lift_arg) in H0; auto.
+    do 2 pair_fst_snd_eqns. reflexivity.
   Qed.
 End Liftlift.
 
@@ -511,44 +444,20 @@ Section liftLift.
     Lift_exp e (fst (lift_exp e)) (snd (lift_exp e)).
   Proof.
     intro e; induction e using custom_exp_ind; cbn;
-      repeat destr_lift_exp; cbn in *; auto.
+      repeat let_destr_pair; unravel; auto.
     - constructor. assumption.
-    - destruct
-        (split (shift_pairs shift_exp $ map lift_exp es)) as [es' les] eqn:hes.
-      rewrite split_map in hes.
-      unravel in *. inv hes.
-      assert (h: Forall3
-                   Lift_exp
-                   es
-                   (map fst (map lift_exp es))
-                   (map snd (map lift_exp es))).
-      { clear l.
-        rewrite Forall_forall in H.
-        rewrite Forall3_forall.
-        repeat rewrite map_length.
-        repeat split; try reflexivity.
-        intros n e e' exps he he' hes.
-        pose proof H _ (nth_error_In _ _ he) as h.
-        do 2 rewrite nth_error_map in he',hes.
-        rewrite he in he',hes.
-        cbn in he',hes.
-        inv he'; inv hes.
-        assumption. }
-      rewrite <- combine_map_fst_snd
-        with (l:=map lift_exp es). auto.
+    - rewrite <- combine_map_fst_snd with (l:=map lift_exp es).
+      constructor.
+      do 2 rewrite <- Forall3_map_23.
+      rewrite Forall3_Forall_123. assumption.
   Qed.
 
   Local Hint Resolve lift_Lift_exp : core.
-
-  Ltac solve_aux h :=
-    pose proof f_equal fst h as h1;
-    pose proof f_equal snd h as h2;
-    cbn in *; subst; auto.
   
   Corollary lift_Lift_exp_aux : forall e e' es,
       lift_exp e = (e', es) -> Lift_exp e e' es.
   Proof.
-    intros e e' es h; solve_aux h.
+    intros; pair_fst_snd_eqns; auto.
   Qed.
 
   Local Hint Resolve lift_Lift_exp_aux : core.
@@ -558,7 +467,7 @@ Section liftLift.
       Lift_arg arg (fst (lift_arg arg)) (snd (lift_arg arg)).
   Proof.
     intros [e | e | e]; unravel;
-      destr_lift_exp; cbn; auto.
+      let_destr_pair; cbn; auto.
   Qed.
 
   Local Hint Resolve lift_Lift_arg : core.
@@ -567,7 +476,7 @@ Section liftLift.
       lift_arg arg = (arg', es) ->
       Lift_arg arg arg' es.
   Proof.
-    intros arg arg' es h; solve_aux h.
+    intros; pair_fst_snd_eqns; auto.
   Qed.
 
   Local Hint Resolve lift_Lift_arg_aux : core.
@@ -577,7 +486,7 @@ Section liftLift.
       Lift_trns e (fst (lift_trns e)) (snd (lift_trns e)).
   Proof.
     intros []; unravel;
-      try destr_lift_exp; cbn; auto.
+      try let_destr_pair; cbn; auto.
   Qed.
 
   Local Hint Resolve lift_Lift_trns : core.
@@ -586,34 +495,18 @@ Section liftLift.
       lift_trns e = (e', es) ->
       Lift_trns e e' es.
   Proof.
-    intros e e' es h; solve_aux h.
+    intros; pair_fst_snd_eqns; auto.
   Qed.
 
   Local Hint Resolve lift_Lift_trns_aux : core.
   Local Hint Constructors Lift_call : core.
-
+  Local Hint Resolve lift_A_list_Lift_A_list : core.
+  
   Lemma lift_Lift_call : forall fk,
       Lift_call fk (fst (lift_call fk)) (snd (lift_call fk)).
   Proof.
     intros [f ts [e |] | a cs | extrn mthd ts [e |] | ? ?];
-      unravel; try destr_lift_exp; cbn; auto.
-    destr_lift_exp_list.
-    unfold lift_exp_list in Heqp.
-    destruct (split (shift_pairs shift_exp $ map lift_exp cs))
-      as [es ees] eqn:hsplit.
-    unravel in *.
-    rewrite split_map in hsplit.
-    inv hsplit; inv Heqp.
-    rewrite <- combine_map_fst_snd
-      with (l:=map lift_exp cs).
-    constructor.
-    rewrite Forall3_forall.
-    repeat rewrite map_length.
-    repeat (split; try reflexivity).
-    intros n e e' es he he' hes.
-    do 2 rewrite nth_error_map in he',hes.
-    rewrite he in he',hes. cbn in *.
-    inv he'; inv hes. auto.
+      unravel; try let_destr_pair; cbn; eauto using lift_A_list_Lift_A_list.
   Qed.
 
   Local Hint Resolve lift_Lift_call : core.
@@ -622,7 +515,7 @@ Section liftLift.
       lift_call fk = (fk', es) ->
       Lift_call fk fk' es.
   Proof.
-    intros fk fk' es h. solve_aux h.
+    intros; pair_fst_snd_eqns; auto.
   Qed.
 
   Local Hint Resolve lift_Lift_call_aux : core.
@@ -632,38 +525,13 @@ Section liftLift.
       Lift_stm s (lift_stm s).
   Proof.
     intro s; induction s; unravel;
-      try destr_lift_trns;
-      repeat destr_lift_exp;
-      try destr_call_pair lift_call;
-      try destr_lift_args;
-      auto.
+      repeat let_destr_pair;
+      eauto using lift_A_list_Lift_A_list.
     - destruct e as [e |];
-        try destr_lift_exp; auto.
-    - unfold lift_args in Heqp0.
-      destruct (split (shift_pairs shift_arg $ map lift_arg args))
-        as [args' les] eqn:hsplit.
-      unravel in *.
-      rewrite split_map in hsplit.
-      inv hsplit; inv Heqp0.
-      rewrite sublist.length_concat.
-      rewrite shift_pairs_inner_length.
-      rewrite <- sublist.length_concat.
-      rewrite <- combine_map_fst_snd
-        with (l := map lift_arg args) at 4.
-      rewrite <- combine_map_fst_snd
-        with (l := map lift_arg args) at 2.
-      constructor; auto.
-      rewrite Forall3_forall.
-      repeat rewrite map_length.
-      repeat (split; try reflexivity).
-      intros n arg arg' es harg harg' hes.
-      do 2 rewrite nth_error_map in harg',hes.
-      unfold Exp.arg in *.
-      rewrite harg in harg',hes; cbn in *.
-      inv harg'; inv hes. auto.
+        try let_destr_pair; auto.
     - destruct lhs as [e |];
-        try destr_lift_exp; eauto.
+        try let_destr_pair; eauto.
     - destruct init as [t | e];
-        try destr_lift_exp; auto.
+        try let_destr_pair; auto.
   Qed.
 End liftLift.
